@prefix rdf:          <http://www.w3.org/1999/02/22-rdf-syntax-ns#> .
@prefix rdfs:         <http://www.w3.org/2000/01/rdf-schema#> .
@prefix dcterms:      <http://purl.org/dc/terms/> .
@prefix skos:         <http://www.w3.org/2004/02/skos/core#> .
@prefix voaf:         <http://purl.org/vocommons/voaf#> .
@prefix vann:         <http://purl.org/vocab/vann/> .
@prefix dbr:          <https://dbpedia.org/resource/> .
@prefix wikidata:     <https://www.wikidata.org/entity/> .
@prefix xsd:          <http://www.w3.org/2001/XMLSchema#> .
@prefix ppfa:         <http://w3id.org/drk/vocabs/personal-profile-for-accessibility#> .

ppfa:
    a                             voaf:Vocabulary, skos:ConceptScheme ;
    dcterms:title                 "Personal Profile for Accessibility Vocabulary"@en ;
    dcterms:description           "A controlled vocabulary for identifying and describing personal profiles from a disability perspective, aimed at facilitating accessibility."@en ;
    rdfs:label                    "Personal Profile for Accessibility Vocabulary"@en ;
    rdfs:comment                  "A controlled vocabulary for identifying and describing personal profiles from a disability perspective, aimed at facilitating accessibility."@en ;
    dcterms:hasVersion            "0.0.1"^^xsd:string ;
    vann:preferredNamespacePrefix "ppfa" ;
    vann:preferredNamespaceUri    "http://w3id.org/drk/vocabs/personal-profile-for-accessibility#" ;
    dcterms:source                <https://sozialhelden.github.io/a11yjson/describing-objects/0-model/#personalprofile> ;
    rdfs:seeAlso                  <https://sozialhelden.github.io/a11yjson/describing-objects/0-model/> .

# See also ppfa:VisualImpairment
ppfa:Blindness
    a               skos:Concept ;
    skos:inScheme   ppfa: ;
    rdfs:label      "Blindness"@en ;
    rdfs:comment    "A term that describes the profile of a person who is blind."@en ;
    skos:closeMatch wikidata:Q10874 .

ppfa:GuideDog
    a               skos:Concept ;
    skos:inScheme   ppfa: ;
    rdfs:label      "Guide Dog"@en ;
    rdfs:comment    "A term that describes the profile of a person who needs a guide dog."@en ;
    skos:closeMatch dbr:Guide_dog, wikidata:Q38782 .

ppfa:HearingImpairment
    a               skos:Concept ;
    skos:inScheme   ppfa: ;
    rdfs:label      "Hearing Impairment"@en ;
    rdfs:comment    "A term that describes the profile of a person who has a hearing impairment."@en ;
    skos:closeMatch dbr:Hearing_impairment, wikidata:Q16035842 .

ppfa:LearningImpairment
    a               skos:Concept ;
    skos:inScheme   ppfa: ;
    rdfs:label      "Learning Impairment"@en ;
    rdfs:comment    "A term that describes the profile of a person who has a learning impairment."@en ;
    skos:closeMatch dbr:Learning_impairment .

ppfa:MobilityImpairment
    a               skos:Concept ;
    skos:inScheme   ppfa: ;
    rdfs:label      "Mobility Impairment"@en ;
    rdfs:comment    "A term that describes the profile of a person who has a mobility impairment."@en ;
    skos:closeMatch dbr:Mobility_impairment, wikidata:Q3317681 .

ppfa:Muteness
    a               skos:Concept ;
    skos:inScheme   ppfa: ;
    rdfs:label      "Muteness"@en ;
    rdfs:comment    "A term that describes the profile of a person who is unable to speak."@en ;
    skos:closeMatch dbr:Muteness, wikidata:Q671776 .

# See also ppfa:Blindness
ppfa:VisualImpairment
    a               skos:Concept ;
    skos:inScheme   ppfa: ;
    rdfs:label      "Visual Impairment"@en ;
    rdfs:comment    "A term that describes the profile of a person who has a visual impairment."@en ;
    skos:exactMatch dbr:Visual_impairment, wikidata:Q737460 .

ppfa:Wheelchair
    a               skos:Concept ;
    skos:inScheme   ppfa: ;
    rdfs:label      "Wheelchair"@en ;
    rdfs:comment    "A term that describes the profile of a person who uses a wheelchair."@en ;
    skos:closeMatch dbr:Wheelchair, wikidata:Q191931 .
