@prefix rdf:          <http://www.w3.org/1999/02/22-rdf-syntax-ns#> .
@prefix rdfs:         <http://www.w3.org/2000/01/rdf-schema#> .
@prefix dcterms:      <http://purl.org/dc/terms/> .
@prefix skos:         <http://www.w3.org/2004/02/skos/core#> .
@prefix voaf:         <http://purl.org/vocommons/voaf#> .
@prefix wikidata:     <https://www.wikidata.org/entity/> .
@prefix vann:         <http://purl.org/vocab/vann/> .
@prefix xsd:          <http://www.w3.org/2001/XMLSchema#> .
@prefix tprod:        <http://w3id.org/drk/vocabs/theatrical-production-types#> .

tprod:
    a                             voaf:Vocabulary, skos:ConceptScheme ;
    dcterms:title                 "Theatrical Production Types Vocabulary"@en ;
    dcterms:description           "A controlled vocabulary for listing and describing theatrical production types."@en ;
    rdfs:label                    "Theatrical Production Types Vocabulary"@en ;
    rdfs:comment                  "A controlled vocabulary for listing and describing theatrical production types."@en ;
    dcterms:hasVersion            "0.0.1"^^xsd:string ;
    vann:preferredNamespacePrefix "tprod" ;
    vann:preferredNamespaceUri    "http://w3id.org/drk/vocabs/theatrical-production-types#" .

tprod:WorldPremiere
    a               skos:Concept ;
    skos:inScheme   tprod: ;
    rdfs:label      "World Premiere"@en, "Uraufführung"@de ;
    skos:altLabel   "World Première"@en, "Weltpremiere"@de, "Welturaufführung"@de ;
    rdfs:comment    "The first public performance of a theatrical creative work such as a play, opera, ballet, etc., in the world."@en ;
    skos:exactMatch wikidata:Q2500107 ;
    rdfs:seeAlso    <https://en.wikipedia.org/wiki/World_Premiere> .

tprod:Revival
    a               skos:Concept ;
    skos:inScheme   tprod: ;
    rdfs:label      "Revival"@en, "Wiederaufnahme"@de ;
    rdfs:comment    "A new production (restaging) of an old play or similar creative work."@en ;
    skos:exactMatch wikidata:Q2568341 ;
    rdfs:seeAlso    <https://en.wikipedia.org/wiki/Revival_(theatre)> .

tprod:LanguagePremiere
    a               skos:Concept ;
    skos:inScheme   tprod: ;
    rdfs:label      "Language Premiere"@en, "Erstaufführung (in einer bestimmten Sprache)"@de ;
    skos:altLabel   "Language Première"@en ;
    rdfs:comment    "The first performance of a play or similar creative work in a particular language."@en ;
    skos:exactMatch wikidata:Q40248002 .

tprod:LocalPremiere
    a               skos:Concept ;
    skos:inScheme   tprod: ;
    rdfs:label      "Local Premiere"@en, "Erstaufführung (in Bezug auf einen Ort oder eine Region)"@de ;
    skos:altLabel   "Local Première"@en ;
    rdfs:comment    "The first performance of a play or similar creative work in a particular local area."@en ;
    skos:exactMatch wikidata:Q40249084 .

tprod:CountryPremiere
    a               skos:Concept ;
    skos:inScheme   tprod: ;
    rdfs:label      "Country Premiere"@en, "Erstaufführung (in einem bestimmten Land)"@de ;
    skos:altLabel   "Country Première"@en ;
    rdfs:comment    "The first performance of a play or similar creative work in a particular country."@en ;
    skos:exactMatch wikidata:Q40248880 .